HouLean/Meta/TypeEncodingInit.lean
@@ -1,0 +1,8 @@
+import Lean
+
+open Lean
+
+initialize registerTraceClass `HouLean.encodespec
+
+
+register_simp_attr encodespec
